DiagonaLean.lean
@@ -2,3 +2,5 @@ import DiagonaLean.Halt.Basic
 import DiagonaLean.Halt.Encoding
 import DiagonaLean.Halt.Compositions
 import DiagonaLean.Halt.Undecidable
+import DiagonaLean.Rice.Basic
+import DiagonaLean.Rice.EmptyLang
